Now handle parameter passing as a form of declaration, which is nice because it gives me re-use.  Handle sub-typing of pointers to classes by importing Wasserab's definition, and sticking it into nonclass_conversion, which is used for assignment and declaration initialisation.

holsrcs/dynamicsScript.sml
@@ -13,8 +13,10 @@ local open wordsTheory integer_wordTheory finite_mapTheory in end
 
 (* C++ ancestor theories  *)
 open typesTheory memoryTheory expressionsTheory staticsTheory class_infoTheory
-open aggregatesTheory
-local open side_effectsTheory statesTheory operatorsTheory in end
+open aggregatesTheory declaration_dynamicsTheory
+local
+  open side_effectsTheory statesTheory operatorsTheory overloadingTheory
+in end
 
 val _ = new_theory "dynamics";
 
@@ -52,79 +54,6 @@ val valid_econtexts_11 = store_thm(
   "valid_econtexts_11",
   ``!f. valid_econtext f ==> !e1 e2. (f e1 = f e2) = (e1 = e2)``,
   SRW_TAC [][valid_econtext_def] THEN SRW_TAC [][])
-
-(* mark_ref checks whether or not we're trying to read something that has been
-   updated *)
-(* class objects don't turn into rvalues - this changes the way that
-   things happen when class/struct values are returned from objects, but
-   shouldn't make much difference otherwise. *)
-val lval2rval_def = Define`
-  lval2rval (s0,e0,se0) (s,e,se) =
-       (s0 = s) /\
-       ?n t p.
-          (e0 = LVal n t p) /\
-             (~array_type t /\ (!cn. ~(t = Class cn)) /\
-              (?sz. sizeof T (sizeofmap s0) t sz /\
-                    (mark_ref n sz se0 se /\
-                     range_set n sz SUBSET s0.initmap /\
-                     (e = ECompVal (mem2val s0 n sz) t) \/
-                     (~(range_set n sz SUBSET s0.initmap) \/
-                      (!se'. ~(mark_ref n sz se0 se'))) /\
-                     (se = se0) /\ (e = UndefinedExpr)))
-          \/
-              (?sz t' bytes.
-                  (t = Array t' sz) /\ (se0 = se) /\
-                  (SOME bytes = ptr_encode (s,t') (n, default_path t')) /\
-                  (e = ECompVal bytes (Ptr t'))))
-`
-
-(* SANITY *)
-val lval2rval_states_equal = store_thm(
-  "lval2rval_states_equal",
-  ``!s0 ese0 s ese. lval2rval (s0,ese0) (s,ese) ==> (s0 = s)``,
-  SIMP_TAC (srw_ss()) [lval2rval_def,pairTheory.FORALL_PROD]);
-
-(* SANITY *)
-val update_map_over_lval2rval = store_thm(
-  "update_map_over_lval2rval",
-  --`!s0 e0 se0 s e se. lval2rval (s0,e0,se0) (s,e,se) ==>
-                        (se0.update_map = se.update_map)`--,
-  SRW_TAC [][lval2rval_def] THEN
-  FULL_SIMP_TAC (srw_ss()) [side_effectsTheory.mark_ref_def])
-
-(* SANITY *)
-val lval2rval_det = store_thm(
-  "lval2rval_det",
-  ``!se0 s0 e0 se s e.
-       lval2rval (s0, e0, se0) (s, e, se) ==>
-       !se' s' e'.
-          lval2rval (s0, e0, se0) (s', e', se') ==>
-          (s' = s) /\ (e' = e) /\ (se' = se)``,
-  SRW_TAC [][lval2rval_def] THEN
-  FULL_SIMP_TAC (srw_ss()) [] THEN
-  METIS_TAC [sizeof_det, TypeBase.one_one_of ``:'a option``,
-             side_effectsTheory.mark_ref_det])
-
-(* SANITY *)
-val lval2rval_is_lval = store_thm(
-  "lval2rval_is_lval",
-  ``!s0 e0 se0 X.
-      lval2rval (s0, e0, se0) X ==> ?n t p. e0 = LVal n t p``,
-  SIMP_TAC (srw_ss() ++ DNF_ss) [lval2rval_def, pairTheory.FORALL_PROD])
-
-(* SANITY *)
-val lval2rval_ecompval = store_thm(
-  "lval2rval_ecompval",
-  ``!s0 v t se0 X. ~(lval2rval (s0, ECompVal v t, se0) X)``,
-  SIMP_TAC (srw_ss()) [pairTheory.FORALL_PROD, CExpr_distinct,
-                       lval2rval_def]);
-
-(* SANITY *)
-val lval2rval_results = store_thm(
-  "lval2rval_results",
-  ``!X s e se. lval2rval X (s,e,se) ==>
-               (?v t. e = ECompVal v t) \/ (e = UndefinedExpr)``,
-  SIMP_TAC (srw_ss() ++ DNF_ss) [pairTheory.FORALL_PROD, lval2rval_def])
 
 (* an lv-context is a function defining where lvalue to rvalue reduction can
    occur *)
@@ -181,65 +110,6 @@ val valid_fvcontext_def = Define`
       !args. ~(f = \f'. FnApp f' args)
 `
 
-(* malloc s0 ty a is true if a is a valid address for a value of type ty,
-   and is currently unallocated.
-
-   If you are malloc-ing space for a class, then it will be for a most-derived
-   class, which is they there are T's passed to sizeof and align. *)
-val malloc_def = Define`
-  malloc s0 ty a =
-     ?sz aln. sizeof T (sizeofmap s0) ty sz /\
-              align (sizeofmap s0) T ty aln /\
-              DISJOINT s0.allocmap (range_set a sz) /\
-              ~(a = 0) /\ (a MOD aln = 0) /\
-              a + sz <= 2 EXP (CHAR_BIT * ptr_size ty)
-`
-
-val parameter_coerce_def = Define`
-  parameter_coerce (v1,ty1) (v2,ty2) =
-    (integral_type ty1 /\ integral_type ty2 \/
-     (?ty0. {ty1; ty2} = {Ptr Void; Ptr ty0})) /\
-    (?i. (INT_VAL ty1 v1 = SOME i) /\
-         (SOME v2 = REP_INT ty2 i))
-       \/
-    (ty1 = ty2) /\ (v1 = v2)
-`;
-
-
-(* installs values into memory *)
-val rec_i_params_def = Define`
-    (rec_i_params s0 [] vallist s = (vallist = []) /\ (s0 = s)) /\
-    (rec_i_params s0 ((pname, ptype) :: ptl) vallist s =
-       (?a n vval vtype newval vtl rs.
-          ~ref_type ptype /\
-          (vallist = ECompVal vval vtype :: vtl) /\
-          parameter_coerce (vval, vtype) (newval, ptype) /\
-          sizeof T (sizeofmap s0) ptype n /\ malloc s0 ptype a /\
-          (rs = range_set a n) /\
-          rec_i_params
-            (val2mem (s0 with
-                        <| varmap updated_by
-                              (\v. v |+ (Base pname,
-                                         (a, default_path ptype))) ;
-                           typemap updated_by (\t. t |+ (Base pname, ptype));
-                           allocmap updated_by ((UNION) rs);
-                           initmap updated_by ((UNION) rs) |>)
-                     a
-                     newval)
-            ptl vtl s) \/
-       (?a ty p vtl.
-          (vallist = LVal a ty p :: vtl) /\ (ptype = Ref ty) /\
-          rec_i_params
-            (s0 with <| varmap updated_by (\v. v |+ (Base pname, (a, p)));
-                        typemap updated_by (\t. t |+ (Base pname, ty)) |>)
-            ptl vtl s))
-`;
-
-val pass_parameters_def = Define`
-  pass_parameters s0 fnid pv s =
-      rec_i_params s0 ((s0.fnmap ' fnid).parameters) pv s
-`;
-
 (* installing a function - generating an address for it at the same time *)
 val installfn_def = Define`
   installfn s0 ftype retty fnid params body fval s =
@@ -286,39 +156,6 @@ val imemfn_def = Define`
 val install_member_functions_def =
     overload_on ("install_member_functions", ``imemfn``)
 
-(* declaration only.  See
-     - 12.1 p5 for constructors
-     - 12.8 p4-5 for copy constructors
-     - 12.8 p10 for copy assignment constructors
-     - 12.4 p3 for destructors
-             - AMBIGUITY: no spec in standard of what body of implicitly
-                          defined destructor should do
-*)
-(* this declares default special members too *)
-val declare_default_specials_def = Define`
-  define_default_specials info0 =
-    let constructor (i0,set) =
-      if (?ps mems bdy statp prot.
-            MEM (Constructor ps mems bdy, statp, prot) i0.fields)
-      then (i0, DefaultConstructor INSERT set)
-      else (i0 with fields updated_by
-                      CONS (Constructor [] [] NONE, F, Public),
-            set) in
-    let destructor (i0,set) =
-      if (?bdy statp prot. MEM (Destructor bdy, statp, prot) i0.fields) then
-        (i0,Destructor INSERT set)
-      else (i0 with fields updated_by CONS (Destructor NONE, F, Public),
-            set)
-    in
-      constructor (destructor (info0, {}))
-`
-
-
-
-
-val _ = overload_on ("mExpr", ``statements$NormE``)
-val _ = overload_on ("mStmt", ``statements$EStmt``)
-
 val signed_int_def = Define`
   signed_int i = THE (REP_INT (Signed Int) i)
 `
@@ -351,36 +188,6 @@ val final_value_def = Define`
   (final_value (mStmt s c) = F)
 `;
 
-val vdeclare_def = Define`
-  vdeclare s0 ty nm s =
-     (?a sz rs.
-         (rs = range_set a sz) /\
-         object_type ty /\ malloc s0 ty a /\ sizeof T (sizeofmap s) ty sz /\
-         (s = s0 with <| allocmap updated_by (UNION) rs;
-                          varmap updated_by
-                             (\vm. vm |+ (nm,(a,default_path ty)));
-                          typemap updated_by (\tm. tm |+ (nm,ty)) |>))
-        \/
-     (function_type ty /\
-      (s = s0 with typemap updated_by (\tm. tm |+ (nm, ty))))
-        \/
-     (?ty0.
-        (ty = Ref ty0) /\
-        (* before the reference gets initialised, what should its value be?
-           Or, what does an uninitialised reference what look like?
-           Certainly, references must be initialised by valid objects, so
-           attempting
-              int &y = y ;
-           must be bad.  So, let's make it a reference to a guaranteed bad
-           address, 0.  We can't just leave the varmap unchanged as
-           the declaration of a variable masks other variables of the same
-           name.  See notes/ref001.cpp *)
-        (s = s0 with
-             <| varmap updated_by (\vm. vm |+ (nm, (0, default_path ty0)));
-                typemap updated_by (\tm. tm |+ (nm, ty0)) |>))
-
-`;
-
 val copy2globals_def = Define`
   copy2globals s = (s with <| gclassmap := s.classmap;
                               gtypemap := s.typemap;
@@ -397,9 +204,7 @@ val fn_expects_rval_def = Define`
       ~ref_type (EL n args)
 `;
 
-(* true if the nth argument of the constructor for cnm is not a reference
-   type - the actual arguments are passed so that we have a hope of figuring
-   out which actual constructor is going to get called *)
+
 (* TODO: deal with overloading *)
 (* TODO: complete definition of constructor_expects_rval *)
 val constructor_expects_rval_def = Define`
@@ -426,138 +231,6 @@ val find_destructor_info_def = Define`
        MEM (Destructor (SOME body), F, prot) (cinfo s0 cnm).fields
 `;
 
-
-
-val initA_constructor_call_def = Define`
-  initA_constructor_call mdp cnm addr args =
-      VDecInitA (Class cnm)
-                (ObjPlace addr)
-                (DirectInit
-                   (mExpr (FnApp (ConstructorFVal mdp addr cnm) args) base_se))
-`;
-
-
-(* 8.5 p5 : zero-initialisation *)
-(* TODO: handle unions *)
-val (zero_init_rules, zero_init_ind, zero_init_cases) = Hol_reln`
-   (!s mdp ty a.
-     scalar_type ty
-   ==>
-     zero_init s mdp ty a [VDecInitA ty
-                                     (ObjPlace a)
-                                     (DirectInit (mExpr (Cnum 0) base_se))])
-
-   /\
-
-   (!s mdp ty a.
-     ref_type ty
-   ==>
-     zero_init s mdp ty a [])
-
-   /\
-
-   (!s mdp cnm a sub_inits.
-     listRel (\(cc,off) l. zero_init s (nsdp cc) (cc_type cc) (a + off) l)
-             (init_order_offsets s mdp cnm)
-             sub_inits
-   ==>
-     zero_init s mdp (Class cnm) a (FLAT sub_inits))
-
-   /\
-
-   (!s mdp ty n a sz sub_inits.
-     sizeof T (sizeofmap s) ty sz /\
-     listRel (\m l. zero_init s mdp ty (a + m * sz) l)
-             (GENLIST I n)
-             sub_inits
-   ==>
-     zero_init s mdp (Array ty n) a (FLAT sub_inits))
-`;
-
-(* 8.5 p5 : default-initialisation *)
-(* TODO: handle unions *)
-val (default_init_rules, default_init_ind, default_init_cases) = Hol_reln`
-   (!s mdp cnm a.
-     ~PODstruct s cnm
-   ==>
-     default_init s mdp (Class cnm) a [initA_constructor_call mdp cnm a []])
-
-   /\
-
-   (!s mdp ty n a sz sub_inits.
-     sizeof T (sizeofmap s) ty sz /\
-     listRel (\m l. default_init s mdp ty (a + m * sz) l)
-             (GENLIST I n)
-             sub_inits
-   ==>
-     default_init s mdp (Array ty n) a (FLAT sub_inits))
-
-   /\
-
-   (!s mdp ty a inits.
-     ~array_type ty /\
-     (!cnm. (ty = Class cnm) ==> PODstruct s cnm) /\
-     zero_init s mdp ty a inits
-   ==>
-     default_init s mdp ty a inits)
-`;
-
-(* 8.5 p5 : value-initialisation *)
-(* AMBIGUITY: (??)
-    What is the order that the non-static data members and base-class
-    components are initialised in?  It looks to be (literally) unspecified.
-    Or should 12.6.2 p5 take precedence, though it is about
-    the situation where we are inside a constructor call and looking at
-    mem-initializers.  Think so.
-
-    Similarly, it is not specified that arrays should be
-    value-initialised in index order.  BUT, 12.6 does say that arrays
-    of (and presumably, arrays of arrays of) class objects should be
-    initialised in index order.  It is only initialisation of classes
-    that can make any difference (through calls to constructors, so we
-    can value-initialise all arrays in index order).
-
-    Used in initialisation of aggregates: 8.5.1 p7 (see also 12.6.1)
-    Used when a mem-initializer mentions a constituent, but doesn't pass any
-    paramters (12.6.2 p3)
-*)
-(* TODO: handle unions *)
-val (value_init_rules, value_init_ind, value_init_cases) = Hol_reln`
-   (!s mdp cnm addr.
-     has_user_constructor s cnm
-   ==>
-     value_init s mdp (Class cnm) addr
-                [initA_constructor_call mdp cnm addr []])
-
-   /\
-
-   (!s mdp cnm a sub_inits.
-     ~has_user_constructor s cnm /\
-     listRel (\(cc,off) l.
-                value_init s (nsdp cc) (cc_type cc) (a + off) l)
-             (init_order_offsets s mdp cnm)
-             sub_inits
-   ==>
-     value_init s mdp (Class cnm) a (FLAT sub_inits))
-
-   /\
-
-   (!s mdp ty n addr sz sub_inits.
-     sizeof T (sizeofmap s) ty sz /\
-     listRel (\n l. value_init s T ty (addr + n * sz) l)
-             (GENLIST I n)
-             sub_inits
-   ==>
-     value_init s mdp (Array ty n) addr (FLAT sub_inits))
-
-   /\
-
-   (!s mdp a ty inits.
-     (!ty0. ~(ty = Class ty0)) /\ ~array_type ty /\
-     zero_init s mdp ty a inits
-   ==>
-     value_init s mdp ty a inits)
-`;
 
 
 (* this function returns the prefix of sub-object constructor calls that must
@@ -620,181 +293,15 @@ val RVR_def = Define`
   (RVR (mStmt s c) = mStmt s c)
 `
 
-val _ = print "Defining (utility) declaration relation\n"
-(* this relation performs the various manipulations on declaration syntax
-   that are independent of the rest of the meaning relation *)
-(* TODO: handle construction of arrays of objects, which happens in order
-   of increasing subscripts (see 12.6 p3) *)
-val (declmng_rules, declmng_ind, declmng_cases) = Hol_reln`
-
-(* RULE-ID: decl-vdec-nonclass *)
-(!s0 ty name s.
-     vdeclare s0 ty name s /\ object_type ty /\ (!cnm. ~(ty = Class cnm))
-   ==>
-     declmng mng vdf (VDec ty name, s0) ([], vdf s))
-
-   /\
-
-(* RULE-ID: decl-vdec-class *)
-(* if called on to declare a class variable, then the default, argument-less
-   constructor gets called *)
-(!s0 name cnm.
-     T
-   ==>
-     declmng mng vdf (VDec (Class cnm) name, s0)
-             ([VDecInit (Class cnm) name (DirectInit0 [])], s0))
-
-   /\
-
-
-(* decl-vdecinit-start-evaluate rules switche from VDecInit to
-   VDecInitA, reflecting allocation of space for the "object".  The
-   vdeclare relation handles functions and references as well.
-   Functions can't be initialised, so they won't appear here.
-   References must be initialised, and the behaviour of vdeclare on
-   references is to put them into the typemap, but to allocate no
-   space, and to put them into the varmap at address 0.
-
-   This is also the point where the class construction has to be recorded
-   in the blockclasses stack so that destructors will get called in the
-   appropriate reverse order.
-*)
-
-
-(* RULE-ID: decl-vdecinit-start-evaluate-direct-class *)
-(!s0 ty cnm name args s1 s2 a pth.
-     (ty = Class cnm) /\
-     vdeclare s0 ty name s1 /\
-     ((a,pth) = s1.varmap ' name) /\
-     update_blockclasses s1 a cnm s2
-   ==>
-     declmng mng
-             vdf
-             (VDecInit ty name (DirectInit0 args), s0)
-             ([VDecInitA ty
-                         (ObjPlace a)
-                         (DirectInit (mExpr
-                                        (FnApp (ConstructorFVal T a cnm) args)
-                                        base_se))], vdf s2))
-
-   /\
-
-(* RULE-ID: decl-vdecinit-start-evaluate-direct-nonclass *)
-(* A direct initialisation of a non-class object is the same as a
-   copy-initialisation *)
-(!s0 ty name arg s a pth loc.
-     (!cnm. ~(ty = Class cnm)) /\
-     vdeclare s0 ty name s /\
-     ((a,pth) = s.varmap ' name) /\
-     (loc = if ref_type ty then RefPlace NONE name else ObjPlace a)
-   ==>
-     declmng mng
-             vdf
-             (VDecInit ty name (DirectInit0 [arg]), s0)
-             ([VDecInitA ty loc (CopyInit (mExpr arg base_se))], vdf s))
-
-   /\
-
-(* RULE-ID: decl-vdecinit-start-evaluate-copy *)
-(!s0 ty name arg s a pth loc.
-     vdeclare s0 ty name s /\
-     ((a,pth) = s.varmap ' name) /\
-     (loc = if ref_type ty then RefPlace NONE name else ObjPlace a)
-   ==>
-     declmng mng
-             vdf
-             (VDecInit ty name (CopyInit arg), s0)
-             ([VDecInitA ty loc (CopyInit arg)], vdf s))
-
-   /\
-
-
-(* RULE-ID: decl-vdecinit-evaluation *)
-(!s0 ty loc exte exte' s f.
-     mng exte s0 (s, exte') /\
-     ((f = CopyInit) \/ (f = DirectInit))
-   ==>
-     declmng mng vdf (VDecInitA ty loc (f exte), s0)
-                     ([VDecInitA ty loc (f exte')], s))
-
-   /\
-
-(* RULE-ID: decl-vdecinit-lval2rval *)
-(!ty loc e0 se0 s0 s e se f.
-     lval2rval (s0,e0,se0) (s,e,se) /\ ~ref_type ty /\
-     ((f = CopyInit) \/ (f = DirectInit))
-   ==>
-     declmng mng vdf (VDecInitA ty loc (f (NormE e0 se0)), s0)
-                     ([VDecInitA ty loc (f (NormE e se))], s))
-
-   /\
-
-(* RULE-ID: decl-vdecinit-finish *)
-(* for non-class, non-reference types *)
-(!s0 s v ty dty v' se a rs f.
-     parameter_coerce (v,ty) (v',dty) /\
-     is_null_se se /\
-     (!cnm. ~(dty = Class cnm)) /\
-     (s = val2mem (s0 with initmap updated_by (UNION) rs) a v') /\
-     (rs = range_set a (LENGTH v')) /\
-     ((f = CopyInit) \/ (f = DirectInit))
-   ==>
-     declmng mng vdf (VDecInitA dty
-                                (ObjPlace a)
-                                (f (NormE (ECompVal v ty) se)), s0)
-                     ([], s))
-
-   /\
-
-(* RULE-ID: decl-vdecinit-finish-ref *)
-(* a0 is bogus, NULL even. - assume for the moment that aopt doesn't matter *)
-(!s0 ty1 nm a aopt ty2 p s se f.
-     is_null_se se /\
-     ((f = CopyInit) \/ (f = DirectInit)) /\
-     (s = s0 with varmap updated_by (\fm. fm |+ (nm, (a,p))))
-   ==>
-     declmng mng
-             vdf
-             (VDecInitA (Ref ty1)
-                        (RefPlace aopt nm)
-                        (f (NormE (LVal a ty2 p) se)), s0)
-             ([], s))
-
-   /\
-
-(* RULE-ID: decl-vdecinit-direct-class-finish *)
-(* differences with decl-vdecinit-finish:
-     * no need to update memory, or init_map as this will have all been
-       done by the constructor
-*)
-(!cnm a ty se0 s0.
-     is_null_se se0
-   ==>
-     declmng mng vdf
-             (VDecInitA (Class cnm)
-                        (ObjPlace a)
-                        (DirectInit (NormE (ECompVal [] ty) se0)), s0)
-             ([], s0))
-
-(* TODO: add a rule for performing class based CopyInit updates *)
-`
-
-val declmng_MONO = store_thm(
-  "declmng_MONO",
-  ``(!x y z. P x y z ==> Q x y z) ==>
-    (declmng P f s1 s2 ==> declmng Q f s1 s2)``,
-  STRIP_TAC THEN MAP_EVERY Q.ID_SPEC_TAC [`s2`, `s1`] THEN
-  HO_MATCH_MP_TAC declmng_ind THEN SIMP_TAC (srw_ss()) [declmng_rules] THEN
-  REPEAT STRIP_TAC THEN
-  FIRST (map (fn th => MATCH_MP_TAC th THEN SRW_TAC [][] THEN METIS_TAC [])
-             (CONJUNCTS
-                (SIMP_RULE pure_ss [FORALL_AND_THM] declmng_rules))));
-val _ = export_mono "declmng_MONO"
-
 val _ = print "About to define meaning relation\n"
 val mng  =
     mk_var("meaning", ``:ExtE -> CState -> (CState # ExtE) -> bool``)
 val _ = temp_overload_on("ev", ``mExpr``)
+
+val valuetype_def = Define`
+  (valuetype (ECompVal v t) = t) /\
+  (valuetype (LVal a t p) = static_type (t,p))
+`;
 
 
 val (meaning_rules, meaning_ind, meaning_cases) = Hol_reln`
@@ -822,8 +329,9 @@ val (meaning_rules, meaning_ind, meaning_cases) = Hol_reln`
      T
    ==>
      ^mng (mExpr (Cnullptr t) se) s
-          (s, ev (ECompVal (THE (ptr_encode (s,t) (0, default_path t)))
-                            (Ptr t)) se))
+          (s, ev (ECompVal (THE (ptr_encode s 0 t (default_path t)))
+                           (Ptr t))
+                 se))
 
    /\
 
@@ -1058,17 +566,20 @@ val (meaning_rules, meaning_ind, meaning_cases) = Hol_reln`
 
 (* RULE-ID: deref-objptr *)
 (* 5.3.1 p1 - pointer to an object type *)
-(!mval t se s addr pth.
-     object_type t /\ (SOME (addr,pth) = ptr_decode(s,t) mval)
+(!mval t t' se s addr pth.
+     object_type t /\ (SOME mval = ptr_encode s addr t' pth) /\
+     (static_type (t',pth) = t)
    ==>
      ^mng (mExpr (Deref (ECompVal mval (Ptr t))) se) s
-          (s, ev (LVal addr t pth) se))
+          (s, ev (LVal addr t' pth) se))
 
    /\
 
 (* RULE-ID: deref-objptr-fails *)
 (!mval t se s.
-     object_type t /\ (ptr_decode(s,t) mval = NONE)
+     object_type t /\
+     ((!addr t' p. ~(SOME mval = ptr_encode s addr t' p)) \/
+      (?t' p. SOME mval = ptr_encode s 0 t' p))
    ==>
      ^mng (mExpr (Deref (ECompVal mval (Ptr t))) se) s
           (s, ev UndefinedExpr se))
@@ -1090,7 +601,7 @@ val (meaning_rules, meaning_ind, meaning_cases) = Hol_reln`
 (*   TODO: taking the address of a qualified-id, thereby generating
                 a pointer to member *)
 (!a t pth se s result.
-     (SOME result = ptr_encode (s,t) (a,pth))
+     (SOME result = ptr_encode s a t pth)
    ==>
      ^mng (mExpr (Addr (LVal a t pth)) se) s
            (s, ev (ECompVal result (Ptr (static_type (t,pth)))) se))
@@ -1105,7 +616,7 @@ val (meaning_rules, meaning_ind, meaning_cases) = Hol_reln`
      (s.classmap ' cname = SOME (cinfo, userdefs)) /\
      MEM (FldDecl fldname ty, T, prot) cinfo.fields /\
      (s.varmap ' (Member cname fldname) = (addr, pth)) /\
-     (SOME ptrval = ptr_encode (s,ty) (addr,pth))
+     (SOME ptrval = ptr_encode s addr ty pth)
    ==>
      ^mng (mExpr (MemAddr cname fldname) se) s
           (s, ev (ECompVal ptrval (Ptr ty)) se))
@@ -1130,11 +641,12 @@ val (meaning_rules, meaning_ind, meaning_cases) = Hol_reln`
    classes, perhaps by writing an auxiliary relation that does just this
 *)
 (!s v0 t0 v lhs_t se0 se a resv.
-    parameter_coerce (v0,t0) (v,lhs_t) /\
-    (se = add_se (a, v) se0) /\ (resv = ECompVal v lhs_t)
+    ~class_type lhs_t /\
+    (nonclass_conversion s (v0,t0) (v,lhs_t) /\ (* 5.17 p3 *)
+     (se = add_se (a, v) se0) /\ (resv = ECompVal v lhs_t)
                           \/
-    (!v. ~parameter_coerce (v0, t0) (v, lhs_t)) /\
-    (resv = UndefinedExpr) /\ (se = se0)
+     (!v. ~nonclass_conversion s (v0, t0) (v, lhs_t)) /\
+     (resv = UndefinedExpr) /\ (se = se0))
    ==>
      ^mng (mExpr (Assign NONE (LVal a lhs_t []) (ECompVal v0 t0)) se0)
           s (s, ev resv se))
@@ -1144,13 +656,13 @@ val (meaning_rules, meaning_ind, meaning_cases) = Hol_reln`
 (* RULE-ID: postinc *)
 (!se0 se s t t' sz v nv nv1 a resv.
      sizeof T (sizeofmap s) t sz /\ (v = mem2val s a sz) /\
-     range_set a sz SUBSET s.initmap /\
+     range_set a sz SUBSET s.initmap /\ ~class_type t /\
      binop_meaning s CPlus v t (signed_int 1) (Signed Int) nv1 t' /\
-     parameter_coerce (nv1,t') (nv,t) /\
-     (se = add_se (a, nv) se0) /\ (resv = ECompVal v t)
+     (nonclass_conversion s (nv1,t') (nv,t) /\
+      (se = add_se (a, nv) se0) /\ (resv = ECompVal v t)
                 \/
-     (!nv. ~parameter_coerce (nv1, t') (nv, t)) /\
-     (se = se0) /\ (resv = UndefinedExpr)
+      (!nv. ~nonclass_conversion s (nv1, t') (nv, t)) /\
+      (se = se0) /\ (resv = UndefinedExpr))
    ==>
      ^mng (mExpr (PostInc (LVal a t [])) se0) s (s, ev resv se))
 
@@ -1158,7 +670,7 @@ val (meaning_rules, meaning_ind, meaning_cases) = Hol_reln`
 
 (* RULE-ID: postinc-fails-inc-or-initialised *)
 (!a t se0 sz s v.
-     sizeof T (sizeofmap s) t sz /\
+     sizeof T (sizeofmap s) t sz /\ ~class_type t /\
      (v = mem2val s a sz) /\
      ((!nv1 t'.
          ~binop_meaning s CPlus v t (signed_int 1) (Signed Int) nv1 t') \/
@@ -1254,30 +766,15 @@ val (meaning_rules, meaning_ind, meaning_cases) = Hol_reln`
 
 (* RULE-ID: global-function-call *)
 (* the NONE as FVal's third argument means this is a global function *)
-(!ftype params se s0 s1 fnid rt vs body.
-     (ftype = Function rt vs) /\
-     pass_parameters
-       (s0 with <| classmap := s0.gclassmap ;
-                   typemap := s0.gtypemap ;
-                   varmap := s0.varmap |>)
-       fnid params s1 /\
-     ((s0.fnmap ' fnid).body = body)
+(* TODO: handle return type casting *)
+(!ftype args pdecls params se s0 fnid rtype body.
+     (find_best_fnmatch s0 fnid (MAP valuetype args) rtype params body) /\
+     (pdecls = MAP (\ ((n,ty),a). VDecInit ty (Base n)
+                                              (CopyInit (mExpr a base_se)))
+                   (ZIP (params, args)))
    ==>
-     ^mng (mExpr (FnApp_sqpt (FVal fnid ftype NONE) params) se) s0
-          (s1 with
-            stack updated_by
-                  (CONS (s0.classmap, s0.typemap, s0.varmap, s0.thisvalue)),
-           EStmt body (return_cont se rt)))
-
-   /\
-
-(* RULE-ID: function-call-fails *)
-(* works for both global and member function calls *)
-(!ftype params se s0 fnid copt.
-    (!s. ~pass_parameters s0 fnid params s)
-   ==>
-    ^mng (mExpr (FnApp_sqpt (FVal fnid ftype copt) params) se) s0
-         (s0, ev UndefinedExpr se))
+     ^mng (mExpr (FnApp_sqpt (FVal fnid ftype NONE) args) se) s0
+          (s0, EStmt (Block F pdecls [body]) (return_cont se rtype)))
 
    /\
 
@@ -1288,49 +785,46 @@ val (meaning_rules, meaning_ind, meaning_cases) = Hol_reln`
      TODO: set up class member values as "locals".  I.e., if class C
        has a member x, then x can be directly referred to in the
        class's member functions
+
+     NOTE: the block is "manually" entered, hence its flag being T, so that
+     its internal thisvalue can be set correctly.
 *)
-(!fnid ftype a cname args rt se0 s0 s1 p body this.
-     pass_parameters
-       (s0 with <| classmap := s0.gclassmap ;
-                   typemap := s0.gtypemap ;
-                   varmap := s0.varmap |>)
-       fnid args s1 /\
-     ((s0.fnmap ' fnid).body = body) /\
-     (SOME this = ptr_encode (s0, Class cname) (a,p))
+(!fnid ftype a cname args rtype se0 s0 p params pdecls body this.
+     (find_best_fnmatch s0 fnid (MAP valuetype args) rtype params body) /\
+     (pdecls = MAP (\ ((n,ty),a). VDecInit ty (Base n)
+                                              (CopyInit (mExpr a base_se)))
+                   (ZIP (params, args))) /\
+     (SOME this = ptr_encode s0 a (Class cname) p)
    ==>
      ^mng (mExpr (FnApp_sqpt (FVal fnid ftype (SOME (LVal a (Class cname) p)))
                              args) se0)
           s0
-          (s1 with <| stack updated_by
+          (s0 with <| stack updated_by
                         (CONS (s0.classmap,s0.typemap,s0.varmap,s0.thisvalue));
                       thisvalue := SOME (ECompVal this (Ptr (Class cname)));
                       blockclasses updated_by stackenv_newscope
                    |>,
-           EStmt body (return_cont se0 rt)))
+           EStmt (Block T pdecls [body]) (return_cont se0 rtype)))
 
    /\
 
 (* RULE-ID: constructor-function-call *)
-(!cnm mdp a args se0 params s0 s1 mem_inits this body cpfx.
+(!cnm mdp pdecls a args se0 params s0 mem_inits this body cpfx.
      find_constructor_info s0 cnm args params mem_inits body /\
-     rec_i_params
-       (s0 with <| classmap := s0.gclassmap ;
-                   typemap := s0.gtypemap ;
-                   varmap := s0.varmap |>)
-       params
-       args
-       s1 /\
-     (SOME this = ptr_encode (s0, Class cnm) (a, [cnm])) /\
+     (pdecls = MAP (\ ((n,ty),a). VDecInit ty (Base n)
+                                              (CopyInit (mExpr a base_se)))
+                   (ZIP (params, args))) /\
+     (SOME this = ptr_encode s0 a (Class cnm) [cnm]) /\
      (cpfx = construct_ctor_pfx s0 mdp a cnm mem_inits body)
    ==>
      ^mng (mExpr (FnApp_sqpt (ConstructorFVal mdp a cnm) args) se0)
           s0
-          (s1 with <| stack updated_by
+          (s0 with <| stack updated_by
                         (CONS (s0.classmap,s0.typemap,s0.varmap,s0.thisvalue));
                       thisvalue := SOME (ECompVal this (Ptr (Class cnm)));
                       blockclasses updated_by stackenv_newscope
                    |>,
-           EStmt (Block T cpfx [body]) (return_cont se0 Void)))
+           EStmt (Block T (pdecls ++ cpfx) [body]) (return_cont se0 Void)))
 
    /\
 
@@ -1511,7 +1005,9 @@ val (meaning_rules, meaning_ind, meaning_cases) = Hol_reln`
      T
    ==>
      ^mng (mStmt (Block F vds sts) c) s
-          (s with stack updated_by (CONS (s.classmap,s.typemap,s.varmap,NONE)),
+          (s with <| stack updated_by
+                          (CONS (s.classmap,s.typemap,s.varmap,s.thisvalue));
+                     blockclasses updated_by stackenv_newscope |>,
            mStmt (Block T vds sts) c))
 
    /\
@@ -1531,7 +1027,7 @@ val (meaning_rules, meaning_ind, meaning_cases) = Hol_reln`
 (* RULE-ID: destructor-call *)
 (!a p se0 s0 this cnm body.
      (cnm = LAST p) /\ is_null_se se0 /\
-     (SOME this = ptr_encode (s0, Class cnm) (a, [cnm])) /\
+     (SOME this = ptr_encode s0 a (Class cnm) [cnm]) /\
      find_destructor_info s0 cnm body
    ==>
      ^mng (mExpr (DestructorCall a cnm) se0)
