holsrcs/declaration_dynamicsScript.sml
@@ -1,0 +1,497 @@
+(* Dynamic Semantics of C++ forms *)
+
+(* Michael Norrish *)
+
+(* pro-forma *)
+open HolKernel boolLib Parse bossLib BasicProvers
+open boolSimps
+
+
+(* Standard HOL ancestory theories *)
+open arithmeticTheory pred_setTheory integerTheory
+local open wordsTheory integer_wordTheory finite_mapTheory in end
+
+(* C++ ancestor theories  *)
+open typesTheory memoryTheory expressionsTheory staticsTheory class_infoTheory
+open aggregatesTheory
+local
+  open side_effectsTheory statesTheory operatorsTheory overloadingTheory
+in end
+
+val _ = new_theory "declaration_dynamics";
+
+val _ = set_trace "inddef strict" 1
+
+val lval2rval_def = Define`
+  lval2rval (s0,e0,se0) (s,e,se) =
+       (s0 = s) /\
+       ?n t p.
+          (e0 = LVal n t p) /\
+             (~array_type t /\ (!cn. ~(t = Class cn)) /\
+              (?sz. sizeof T (sizeofmap s0) t sz /\
+                    (mark_ref n sz se0 se /\
+                     range_set n sz SUBSET s0.initmap /\
+                     (e = ECompVal (mem2val s0 n sz) t) \/
+                     (~(range_set n sz SUBSET s0.initmap) \/
+                      (!se'. ~(mark_ref n sz se0 se'))) /\
+                     (se = se0) /\ (e = UndefinedExpr)))
+          \/
+              (?sz t' bytes.
+                  (t = Array t' sz) /\ (se0 = se) /\
+                  (SOME bytes = ptr_encode s n t' (default_path t')) /\
+                  (e = ECompVal bytes (Ptr t'))))
+`
+
+(* SANITY *)
+val lval2rval_states_equal = store_thm(
+  "lval2rval_states_equal",
+  ``!s0 ese0 s ese. lval2rval (s0,ese0) (s,ese) ==> (s0 = s)``,
+  SIMP_TAC (srw_ss()) [lval2rval_def,pairTheory.FORALL_PROD]);
+
+(* SANITY *)
+val update_map_over_lval2rval = store_thm(
+  "update_map_over_lval2rval",
+  --`!s0 e0 se0 s e se. lval2rval (s0,e0,se0) (s,e,se) ==>
+                        (se0.update_map = se.update_map)`--,
+  SRW_TAC [][lval2rval_def] THEN
+  FULL_SIMP_TAC (srw_ss()) [side_effectsTheory.mark_ref_def])
+
+(* SANITY *)
+val lval2rval_det = store_thm(
+  "lval2rval_det",
+  ``!se0 s0 e0 se s e.
+       lval2rval (s0, e0, se0) (s, e, se) ==>
+       !se' s' e'.
+          lval2rval (s0, e0, se0) (s', e', se') ==>
+          (s' = s) /\ (e' = e) /\ (se' = se)``,
+  SRW_TAC [][lval2rval_def] THEN
+  FULL_SIMP_TAC (srw_ss()) [] THEN
+  METIS_TAC [sizeof_det, TypeBase.one_one_of ``:'a option``,
+             side_effectsTheory.mark_ref_det])
+
+(* SANITY *)
+val lval2rval_is_lval = store_thm(
+  "lval2rval_is_lval",
+  ``!s0 e0 se0 X.
+      lval2rval (s0, e0, se0) X ==> ?n t p. e0 = LVal n t p``,
+  SIMP_TAC (srw_ss() ++ DNF_ss) [lval2rval_def, pairTheory.FORALL_PROD])
+
+(* SANITY *)
+val lval2rval_ecompval = store_thm(
+  "lval2rval_ecompval",
+  ``!s0 v t se0 X. ~(lval2rval (s0, ECompVal v t, se0) X)``,
+  SIMP_TAC (srw_ss()) [pairTheory.FORALL_PROD, CExpr_distinct,
+                       lval2rval_def]);
+
+(* SANITY *)
+val lval2rval_results = store_thm(
+  "lval2rval_results",
+  ``!X s e se. lval2rval X (s,e,se) ==>
+               (?v t. e = ECompVal v t) \/ (e = UndefinedExpr)``,
+  SIMP_TAC (srw_ss() ++ DNF_ss) [pairTheory.FORALL_PROD, lval2rval_def])
+
+(* malloc s0 ty a is true if a is a valid address for a value of type ty,
+   and is currently unallocated.
+
+   If you are malloc-ing space for a class, then it will be for a most-derived
+   class, which is they there are T's passed to sizeof and align. *)
+val malloc_def = Define`
+  malloc s0 ty a =
+     ?sz aln. sizeof T (sizeofmap s0) ty sz /\
+              align (sizeofmap s0) T ty aln /\
+              DISJOINT s0.allocmap (range_set a sz) /\
+              ~(a = 0) /\ (a MOD aln = 0) /\
+              a + sz <= 2 EXP (CHAR_BIT * ptr_size ty)
+`
+
+(* clause 4's conversions, referenced in 8.5 para 14 *)
+(* doesn't include lvalue-to-rvalue conversion - this is handled specially
+    elsewhere because of the restrictions on accessing and reading memory
+    at the same time. *)
+val nonclass_conversion_def = Define`
+  nonclass_conversion s (v1,ty1) (v2,ty2) =
+    (integral_type ty1 /\ integral_type ty2 \/
+     (?ty0. {ty1; ty2} = {Ptr Void; Ptr ty0})) /\
+    (?i. (INT_VAL ty1 v1 = SOME i) /\
+         (SOME v2 = REP_INT ty2 i))
+       \/
+    (ty1 = ty2) /\ (v1 = v2)
+       \/
+    (?c1 c2 addr pth1 pth2.  (* this is an upcast *)
+        (ty1 = Ptr (Class (LAST pth1))) /\ (ty2 = Ptr (Class c2)) /\
+        (SOME v1 = ptr_encode s addr (Class c1) pth1) /\
+        s |- c2 casts pth1 into pth2 /\
+        (SOME v2 = ptr_encode s addr (Class c1) pth2))
+`;
+
+
+(* declaration only.  See
+     - 12.1 p5 for constructors
+     - 12.8 p4-5 for copy constructors
+     - 12.8 p10 for copy assignment constructors
+     - 12.4 p3 for destructors
+             - AMBIGUITY: no spec in standard of what body of implicitly
+                          defined destructor should do
+*)
+(* this declares default special members too *)
+val declare_default_specials_def = Define`
+  define_default_specials info0 =
+    let constructor (i0,set) =
+      if (?ps mems bdy statp prot.
+            MEM (Constructor ps mems bdy, statp, prot) i0.fields)
+      then (i0, DefaultConstructor INSERT set)
+      else (i0 with fields updated_by
+                      CONS (Constructor [] [] NONE, F, Public),
+            set) in
+    let destructor (i0,set) =
+      if (?bdy statp prot. MEM (Destructor bdy, statp, prot) i0.fields) then
+        (i0,Destructor INSERT set)
+      else (i0 with fields updated_by CONS (Destructor NONE, F, Public),
+            set)
+    in
+      constructor (destructor (info0, {}))
+`
+
+
+
+
+val _ = overload_on ("mExpr", ``statements$NormE``)
+val _ = overload_on ("mStmt", ``statements$EStmt``)
+
+val vdeclare_def = Define`
+  vdeclare s0 ty nm s =
+     (?a sz rs.
+         (rs = range_set a sz) /\
+         object_type ty /\ malloc s0 ty a /\ sizeof T (sizeofmap s) ty sz /\
+         (s = s0 with <| allocmap updated_by (UNION) rs;
+                          varmap updated_by
+                             (\vm. vm |+ (nm,(a,default_path ty)));
+                          typemap updated_by (\tm. tm |+ (nm,ty)) |>))
+        \/
+     (function_type ty /\
+      (s = s0 with typemap updated_by (\tm. tm |+ (nm, ty))))
+        \/
+     (?ty0.
+        (ty = Ref ty0) /\
+        (* before the reference gets initialised, what should its value be?
+           Or, what does an uninitialised reference what look like?
+           Certainly, references must be initialised by valid objects, so
+           attempting
+              int &y = y ;
+           must be bad.  So, let's make it a reference to a guaranteed bad
+           address, 0.  We can't just leave the varmap unchanged as
+           the declaration of a variable masks other variables of the same
+           name.  See notes/ref001.cpp *)
+        (s = s0 with
+             <| varmap updated_by (\vm. vm |+ (nm, (0, default_path ty0)));
+                typemap updated_by (\tm. tm |+ (nm, ty0)) |>))
+
+`;
+
+
+val initA_constructor_call_def = Define`
+  initA_constructor_call mdp cnm addr args =
+      VDecInitA (Class cnm)
+                (ObjPlace addr)
+                (DirectInit
+                   (mExpr (FnApp (ConstructorFVal mdp addr cnm) args) base_se))
+`;
+
+
+(* 8.5 p5 : zero-initialisation *)
+(* TODO: handle unions *)
+val (zero_init_rules, zero_init_ind, zero_init_cases) = Hol_reln`
+   (!s mdp ty a.
+     scalar_type ty
+   ==>
+     zero_init s mdp ty a [VDecInitA ty
+                                     (ObjPlace a)
+                                     (DirectInit (mExpr (Cnum 0) base_se))])
+
+   /\
+
+   (!s mdp ty a.
+     ref_type ty
+   ==>
+     zero_init s mdp ty a [])
+
+   /\
+
+   (!s mdp cnm a sub_inits.
+     listRel (\(cc,off) l. zero_init s (nsdp cc) (cc_type cc) (a + off) l)
+             (init_order_offsets s mdp cnm)
+             sub_inits
+   ==>
+     zero_init s mdp (Class cnm) a (FLAT sub_inits))
+
+   /\
+
+   (!s mdp ty n a sz sub_inits.
+     sizeof T (sizeofmap s) ty sz /\
+     listRel (\m l. zero_init s mdp ty (a + m * sz) l)
+             (GENLIST I n)
+             sub_inits
+   ==>
+     zero_init s mdp (Array ty n) a (FLAT sub_inits))
+`;
+
+(* 8.5 p5 : default-initialisation *)
+(* TODO: handle unions *)
+val (default_init_rules, default_init_ind, default_init_cases) = Hol_reln`
+   (!s mdp cnm a.
+     ~PODstruct s cnm
+   ==>
+     default_init s mdp (Class cnm) a [initA_constructor_call mdp cnm a []])
+
+   /\
+
+   (!s mdp ty n a sz sub_inits.
+     sizeof T (sizeofmap s) ty sz /\
+     listRel (\m l. default_init s mdp ty (a + m * sz) l)
+             (GENLIST I n)
+             sub_inits
+   ==>
+     default_init s mdp (Array ty n) a (FLAT sub_inits))
+
+   /\
+
+   (!s mdp ty a inits.
+     ~array_type ty /\
+     (!cnm. (ty = Class cnm) ==> PODstruct s cnm) /\
+     zero_init s mdp ty a inits
+   ==>
+     default_init s mdp ty a inits)
+`;
+
+(* 8.5 p5 : value-initialisation *)
+(* AMBIGUITY: (??)
+    What is the order that the non-static data members and base-class
+    components are initialised in?  It looks to be (literally) unspecified.
+    Or should 12.6.2 p5 take precedence, though it is about
+    the situation where we are inside a constructor call and looking at
+    mem-initializers.  Think so.
+
+    Similarly, it is not specified that arrays should be
+    value-initialised in index order.  BUT, 12.6 does say that arrays
+    of (and presumably, arrays of arrays of) class objects should be
+    initialised in index order.  It is only initialisation of classes
+    that can make any difference (through calls to constructors, so we
+    can value-initialise all arrays in index order).
+
+    Used in initialisation of aggregates: 8.5.1 p7 (see also 12.6.1)
+    Used when a mem-initializer mentions a constituent, but doesn't pass any
+    paramters (12.6.2 p3)
+*)
+(* TODO: handle unions *)
+val (value_init_rules, value_init_ind, value_init_cases) = Hol_reln`
+   (!s mdp cnm addr.
+     has_user_constructor s cnm
+   ==>
+     value_init s mdp (Class cnm) addr
+                [initA_constructor_call mdp cnm addr []])
+
+   /\
+
+   (!s mdp cnm a sub_inits.
+     ~has_user_constructor s cnm /\
+     listRel (\(cc,off) l.
+                value_init s (nsdp cc) (cc_type cc) (a + off) l)
+             (init_order_offsets s mdp cnm)
+             sub_inits
+   ==>
+     value_init s mdp (Class cnm) a (FLAT sub_inits))
+
+   /\
+
+   (!s mdp ty n addr sz sub_inits.
+     sizeof T (sizeofmap s) ty sz /\
+     listRel (\n l. value_init s T ty (addr + n * sz) l)
+             (GENLIST I n)
+             sub_inits
+   ==>
+     value_init s mdp (Array ty n) addr (FLAT sub_inits))
+
+   /\
+
+   (!s mdp a ty inits.
+     (!ty0. ~(ty = Class ty0)) /\ ~array_type ty /\
+     zero_init s mdp ty a inits
+   ==>
+     value_init s mdp ty a inits)
+`;
+
+
+val _ = print "Defining (utility) declaration relation\n"
+(* this relation performs the various manipulations on declaration syntax
+   that are independent of the rest of the meaning relation *)
+(* TODO: handle construction of arrays of objects, which happens in order
+   of increasing subscripts (see 12.6 p3) *)
+val (declmng_rules, declmng_ind, declmng_cases) = Hol_reln`
+
+(* RULE-ID: decl-vdec-nonclass *)
+(!s0 ty name s.
+     vdeclare s0 ty name s /\ object_type ty /\ (!cnm. ~(ty = Class cnm))
+   ==>
+     declmng mng vdf (VDec ty name, s0) ([], vdf s))
+
+   /\
+
+(* RULE-ID: decl-vdec-class *)
+(* if called on to declare a class variable, then the default, argument-less
+   constructor gets called *)
+(!s0 name cnm.
+     T
+   ==>
+     declmng mng vdf (VDec (Class cnm) name, s0)
+             ([VDecInit (Class cnm) name (DirectInit0 [])], s0))
+
+   /\
+
+
+(* decl-vdecinit-start-evaluate rules switche from VDecInit to
+   VDecInitA, reflecting allocation of space for the "object".  The
+   vdeclare relation handles functions and references as well.
+   Functions can't be initialised, so they won't appear here.
+   References must be initialised, and the behaviour of vdeclare on
+   references is to put them into the typemap, but to allocate no
+   space, and to put them into the varmap at address 0.
+
+   This is also the point where the class construction has to be recorded
+   in the blockclasses stack so that destructors will get called in the
+   appropriate reverse order.
+*)
+
+
+(* RULE-ID: decl-vdecinit-start-evaluate-direct-class *)
+(!s0 ty cnm name args s1 s2 a pth.
+     (ty = Class cnm) /\
+     vdeclare s0 ty name s1 /\
+     ((a,pth) = s1.varmap ' name) /\
+     update_blockclasses s1 a cnm s2
+   ==>
+     declmng mng
+             vdf
+             (VDecInit ty name (DirectInit0 args), s0)
+             ([VDecInitA ty
+                         (ObjPlace a)
+                         (DirectInit (mExpr
+                                        (FnApp (ConstructorFVal T a cnm) args)
+                                        base_se))], vdf s2))
+
+   /\
+
+(* RULE-ID: decl-vdecinit-start-evaluate-direct-nonclass *)
+(* A direct initialisation of a non-class object is the same as a
+   copy-initialisation *)
+(!s0 ty name arg s a pth loc.
+     (!cnm. ~(ty = Class cnm)) /\
+     vdeclare s0 ty name s /\
+     ((a,pth) = s.varmap ' name) /\
+     (loc = if ref_type ty then RefPlace NONE name else ObjPlace a)
+   ==>
+     declmng mng
+             vdf
+             (VDecInit ty name (DirectInit0 [arg]), s0)
+             ([VDecInitA ty loc (CopyInit (mExpr arg base_se))], vdf s))
+
+   /\
+
+(* RULE-ID: decl-vdecinit-start-evaluate-copy *)
+(!s0 ty name arg s a pth loc.
+     vdeclare s0 ty name s /\
+     ((a,pth) = s.varmap ' name) /\
+     (loc = if ref_type ty then RefPlace NONE name else ObjPlace a)
+   ==>
+     declmng mng
+             vdf
+             (VDecInit ty name (CopyInit arg), s0)
+             ([VDecInitA ty loc (CopyInit arg)], vdf s))
+
+   /\
+
+
+(* RULE-ID: decl-vdecinit-evaluation *)
+(!s0 ty loc exte exte' s f.
+     mng exte s0 (s, exte') /\
+     ((f = CopyInit) \/ (f = DirectInit))
+   ==>
+     declmng mng vdf (VDecInitA ty loc (f exte), s0)
+                     ([VDecInitA ty loc (f exte')], s))
+
+   /\
+
+(* RULE-ID: decl-vdecinit-lval2rval *)
+(!ty loc e0 se0 s0 s e se f.
+     lval2rval (s0,e0,se0) (s,e,se) /\ ~ref_type ty /\
+     ((f = CopyInit) \/ (f = DirectInit))
+   ==>
+     declmng mng vdf (VDecInitA ty loc (f (NormE e0 se0)), s0)
+                     ([VDecInitA ty loc (f (NormE e se))], s))
+
+   /\
+
+(* RULE-ID: decl-vdecinit-finish *)
+(* for non-class, non-reference types *)
+(!s0 s v ty dty v' se a rs f.
+     nonclass_conversion s0 (v,ty) (v',dty) /\
+     is_null_se se /\
+     (!cnm. ~(dty = Class cnm)) /\
+     (s = val2mem (s0 with initmap updated_by (UNION) rs) a v') /\
+     (rs = range_set a (LENGTH v')) /\
+     ((f = CopyInit) \/ (f = DirectInit))
+   ==>
+     declmng mng vdf (VDecInitA dty
+                                (ObjPlace a)
+                                (f (NormE (ECompVal v ty) se)), s0)
+                     ([], s))
+
+   /\
+
+(* RULE-ID: decl-vdecinit-finish-ref *)
+(* a0 is bogus, NULL even. - assume for the moment that aopt doesn't matter *)
+(!s0 ty1 nm a aopt ty2 p s se f.
+     is_null_se se /\
+     ((f = CopyInit) \/ (f = DirectInit)) /\
+     (s = s0 with varmap updated_by (\fm. fm |+ (nm, (a,p))))
+   ==>
+     declmng mng
+             vdf
+             (VDecInitA (Ref ty1)
+                        (RefPlace aopt nm)
+                        (f (NormE (LVal a ty2 p) se)), s0)
+             ([], s))
+
+   /\
+
+(* RULE-ID: decl-vdecinit-direct-class-finish *)
+(* differences with decl-vdecinit-finish:
+     * no need to update memory, or init_map as this will have all been
+       done by the constructor
+*)
+(!cnm a ty se0 s0.
+     is_null_se se0
+   ==>
+     declmng mng vdf
+             (VDecInitA (Class cnm)
+                        (ObjPlace a)
+                        (DirectInit (NormE (ECompVal [] ty) se0)), s0)
+             ([], s0))
+
+(* TODO: add a rule for performing class based CopyInit updates *)
+`
+
+val declmng_MONO = store_thm(
+  "declmng_MONO",
+  ``(!x y z. P x y z ==> Q x y z) ==>
+    (declmng P f s1 s2 ==> declmng Q f s1 s2)``,
+  STRIP_TAC THEN MAP_EVERY Q.ID_SPEC_TAC [`s2`, `s1`] THEN
+  HO_MATCH_MP_TAC declmng_ind THEN SIMP_TAC (srw_ss()) [declmng_rules] THEN
+  REPEAT STRIP_TAC THEN
+  FIRST (map (fn th => MATCH_MP_TAC th THEN SRW_TAC [][] THEN METIS_TAC [])
+             (CONJUNCTS
+                (SIMP_RULE pure_ss [FORALL_AND_THM] declmng_rules))));
+val _ = export_mono "declmng_MONO"
+
+val _ = export_theory();
+
+
