holsrcs/overloadingScript.sml
@@ -1,0 +1,31 @@
+(* Overloading Resolution for C++ Functions *)
+
+(* Michael Norrish *)
+
+(* pro-forma *)
+open HolKernel boolLib Parse bossLib BasicProvers
+open boolSimps
+
+
+(* Standard HOL ancestory theories *)
+open arithmeticTheory pred_setTheory integerTheory
+local open wordsTheory integer_wordTheory finite_mapTheory in end
+
+(* C++ ancestor theories  *)
+local open side_effectsTheory statesTheory operatorsTheory in end
+
+
+
+val _ = new_theory "overloading"
+
+(* given the state, a function-identifier, and the types of the actual
+   arguments, return ("relationally"), the return type, parameters and
+   body of the function that should be called *)
+val find_best_fnmatch_def = Define`
+  find_best_fnmatch s fnid actualtypes rettype params body =
+    (s.fnmap ' fnid = <| return_type := rettype;
+                         parameters := params;
+                         body := body |>)
+`;
+
+val _ = export_theory()
